\begin{dmath}
\log(Z) = 0
\end{dmath}
\begin{dmath}
R = \frac{1}{{\beta}}
\end{dmath}
\begin{dmath}
KtoL = \left(\frac{{\alpha}}{\frac{1}{{\beta}}-\left(1-{\delta}\right)}\right)^{\frac{1}{1-{\alpha}}}
\end{dmath}
\begin{dmath}
CtoL = {KtoL}^{{\alpha}}-{\delta}\, {KtoL}
\end{dmath}
\begin{dmath}
W = \left(1-{\alpha}\right)\, {KtoL}^{{\alpha}}
\end{dmath}
\begin{dmath}
L = \left({KtoL}^{{\alpha}}\, \frac{\frac{1-{\alpha}}{{\xi}}}{{CtoL}}\right)^{\frac{{\nu}}{1+{\nu}}}
\end{dmath}
\begin{dmath}
K = {KtoL}\, {L}
\end{dmath}
\begin{dmath}
Y = {K}^{{\alpha}}\, {L}^{1-{\alpha}}
\end{dmath}
\begin{dmath}
I = {\delta}\, {K}
\end{dmath}
\begin{dmath}
C = {Y}-{I}
\end{dmath}
